\documentclass{article}
\usepackage{amsmath}
\usepackage[margin=1in]{geometry}

\begin{document}

\section*{Answer Key for Logarithm Practice Problems}

\begin{enumerate}
  \item $\ln(5) + \ln(4) = \ln(20)$
  \item $\ln(7) - \ln(2) = \ln\!\bigl(\tfrac{7}{2}\bigr)$
  \item $2\ln(3) - \ln(6) = \ln(9) - \ln(6) = \ln\!\bigl(\tfrac{9}{6}\bigr) = \ln\!\bigl(\tfrac{3}{2}\bigr)$
  \item $\ln(8) - \ln(2) - \ln(2) = \ln\!\bigl(\tfrac{8}{2\cdot2}\bigr) = \ln(2)$
  \item $\ln(9) + \tfrac12\ln(4) = \ln(9) + \ln(2) = \ln(18)$
  \item $3\ln(2) - \ln(8) = \ln(8) - \ln(8) = 0$
  \item $\ln(5x) - \ln(x) = \ln\!\bigl(\tfrac{5x}{x}\bigr) = \ln(5)$
  \item $\ln\!\bigl(\tfrac{6}{x}\bigr) + \ln(x) = \ln\!\bigl(\tfrac{6}{x}\cdot x\bigr) = \ln(6)$
  \item $\ln(x^2) - 2\ln(x) = \ln(x^2) - \ln(x^2) = 0$
  \item $\ln(3) + \ln(7) - \ln(21) = \ln\!\bigl(\tfrac{3\cdot7}{21}\bigr) = \ln(1) = 0$
  \item $\ln(10) - \ln(2) - \ln(5) = \ln\!\bigl(\tfrac{10}{2\cdot5}\bigr) = \ln(1) = 0$
  \item $2\ln(5) - \ln(25) = \ln(25) - \ln(25) = 0$
  \item $\ln(6) + \ln(2) - \ln(3) = \ln\!\bigl(\tfrac{6\cdot2}{3}\bigr) = \ln(4)$
  \item $\ln(12) - \ln(4) = \ln\!\bigl(\tfrac{12}{4}\bigr) = \ln(3)$
  \item $3\ln(3) - 2\ln(9) = \ln(27) - \ln(81) = \ln\!\bigl(\tfrac{27}{81}\bigr) = \ln\!\bigl(\tfrac13\bigr) = -\ln(3)$
  \item $\ln(18) - \ln(2) - \ln(9) = \ln\!\bigl(\tfrac{18}{2\cdot9}\bigr) = \ln(1) = 0$
  \item $\ln(2x) + \ln(3x) - \ln(6x^2) = \ln\!\bigl(\tfrac{2x\cdot3x}{6x^2}\bigr) = \ln(1) = 0$
  \item $\ln\!\bigl(\tfrac{x^2}{4}\bigr) + \ln(4) = \ln\!\bigl(\tfrac{x^2}{4}\cdot4\bigr) = \ln(x^2) = 2\ln(x)$
  \item $\ln\!\bigl(\tfrac{9}{x}\bigr) + \ln(x) = \ln\!\bigl(\tfrac{9}{x}\cdot x\bigr) = \ln(9)$
  \item $2\ln(7) - \ln(49) = \ln(49) - \ln(49) = 0$
\end{enumerate}

\end{document}
